fixed DevRouter, Arbiter

Arbiter/Impl.v
@@ -155,23 +155,9 @@ Section ArbiterImpl.
            (@FreeList.Ifc.regs numTransactions freelist).
 
     (* TODO: LLEE: check *)
-    Definition regFiles
-      := [
-           {|
-             rfIsWrMask  := false;
-             rfNum       := numTransactions;
-             rfDataArray := alistName;
-             rfRead      := (Async [alistRead]);
-             rfWrite     := alistWrite;
-             rfIdxNum    := numTransactions; (* TODO: LLEE: what does rfIdxNum represent? *)
-             rfData      := ClientIdTag;
-             rfInit
-               := RFNonFile
-                    numTransactions
-                    (Some (getDefaultConst ClientIdTag))
-           |}
-         ] ++
-         (@FreeList.Ifc.regFiles numTransactions freelist).
+    Definition regFiles :=
+      @Build_RegFileBase false 1 alistName (Async [alistRead]) alistWrite numTransactions ClientIdTag (@RFNonFile _ _ None) ::
+                         (@FreeList.Ifc.regFiles numTransactions freelist).
 
     Definition arbiterImpl
       :  Arbiter
