DevRouter/Ifc.v
@@ -25,6 +25,7 @@ Section withParams.
     Class DevRouter : Type :=
       {
         regs: list RegInitT;
+        regFiles: list RegFileBase;
         pollRules (clientCallback: forall {ty}, ty respK -> ActionT ty Void): list (forall {ty}, ActionT ty Void);
         devRouterReq: forall {ty}, ty DevRouterReq -> ActionT ty Bool;
       }.
